

# Tutorial: Gradients, Jacobians & The Trace Trick

Duration: 90 Minutes

## Instructor/TA Note

This tutorial is designed to be extremely granular. Students often get lost in the jump from scalar to matrix notation.

- **Part 1 (Scalar to Vector):** Focus on the mechanics of partial differentiation.
  - **Part 2 (Vector to Vector):** Focus on **Dimensions**. Always ask: "What is the size of the input? What is the size of the output?"
  - **Part 3 (Matrix to Scalar):** Focus on the **Trace Trick**. The goal is to manipulate the differential  $dL$  until it looks like  $\text{tr}(\mathbf{G}^T d\mathbf{X})$ .
- 

## 1 Part 1: Basic Gradient Calculation (Direct Method)

Time Allocation: 20 Minutes

### Problem 1: Gradient of a Quadratic Function

Let  $\mathbf{x} = \begin{bmatrix} x_1 \\ x_2 \end{bmatrix} \in \mathbb{R}^2$ . Consider the scalar function:

$$f(\mathbf{x}) = 3x_1^2 + 2x_1x_2 + x_2^2$$

1. Calculate the gradient vector  $\nabla f(\mathbf{x})$ .
2. Evaluate the gradient at the point  $\mathbf{p} = \begin{bmatrix} 1 \\ -1 \end{bmatrix}$ .

### Detailed Solution:

**Step 1: Understand the Goal** The gradient  $\nabla f(\mathbf{x})$  is a vector that collects all the partial derivatives. Since  $\mathbf{x}$  has 2 components  $(x_1, x_2)$ , the gradient will be a vector of size 2.

$$\nabla f(\mathbf{x}) = \begin{bmatrix} \frac{\partial f}{\partial x_1} \\ \frac{\partial f}{\partial x_2} \end{bmatrix}$$

**Step 2: Compute Partial Derivative w.r.t  $x_1$**  \*Rule:\* When differentiating with respect

to  $x_1$ , treat  $x_2$  as a constant number (like 5 or  $\pi$ ).

$$\begin{aligned}
 f(\mathbf{x}) &= \underbrace{3x_1^2}_{\text{Depends on } x_1} + \underbrace{2x_1x_2}_{\text{Linear in } x_1} + \underbrace{x_2^2}_{\text{Constant w.r.t } x_1} \\
 \frac{\partial f}{\partial x_1} &= \frac{d}{dx_1}(3x_1^2) + \frac{d}{dx_1}(2x_1x_2) + \frac{d}{dx_1}(x_2^2) \\
 &= 6x_1 + 2x_2(1) + 0 \\
 &= 6x_1 + 2x_2
 \end{aligned}$$

**Step 3: Compute Partial Derivative w.r.t  $x_2$**  \*Rule:\* Now treat  $x_1$  as a constant.

$$\begin{aligned}
 f(\mathbf{x}) &= \underbrace{3x_1^2}_{\text{Constant}} + \underbrace{2x_1x_2}_{\text{Linear in } x_2} + \underbrace{x_2^2}_{\text{Depends on } x_2} \\
 \frac{\partial f}{\partial x_2} &= 0 + 2x_1(1) + 2x_2 \\
 &= 2x_1 + 2x_2
 \end{aligned}$$

**Step 4: Assemble the Vector** Stack the results:

$$\nabla f(\mathbf{x}) = \begin{bmatrix} 6x_1 + 2x_2 \\ 2x_1 + 2x_2 \end{bmatrix}$$

**Step 5: Numerical Evaluation** Substitute  $x_1 = 1$  and  $x_2 = -1$ :

$$\nabla f(1, -1) = \begin{bmatrix} 6(1) + 2(-1) \\ 2(1) + 2(-1) \end{bmatrix} = \begin{bmatrix} 6 - 2 \\ 2 - 2 \end{bmatrix} = \begin{bmatrix} 4 \\ 0 \end{bmatrix}$$

\*Interpretation:\* At the point  $(1, -1)$ , the function increases most rapidly in the direction  $(4, 0)$  (purely along the x-axis).

## 2 Part 2: Jacobians & Chain Rule

Time Allocation: 25 Minutes

### Problem 2: The Affine Transformation

Let  $\mathbf{x} \in \mathbb{R}^n$ ,  $\mathbf{W} \in \mathbb{R}^{m \times n}$ , and  $\mathbf{b} \in \mathbb{R}^m$ . Define the function:

$$\mathbf{y} = f(\mathbf{x}) = \mathbf{W}\mathbf{x} + \mathbf{b}$$

1. What are the dimensions of the Jacobian matrix  $\mathbf{J} = \frac{\partial \mathbf{y}}{\partial \mathbf{x}}$ ?
2. Calculate  $\mathbf{J}$  explicitly by analyzing the partial derivative  $\frac{\partial y_i}{\partial x_j}$ .

**Detailed Solution:**

#### 1. Dimension Analysis (Crucial Step):

- **Input:**  $\mathbf{x}$  is a vector of size  $n \times 1$ .
- **Output:**  $\mathbf{y}$  is a vector of size  $m \times 1$ .
- **Definition:** The Jacobian  $\mathbf{J}$  contains the derivative of *every* output component w.r.t *every* input component.
- **Conclusion:** Rows = Output Size ( $m$ ), Columns = Input Size ( $n$ ).  $\mathbf{J}$  is  $m \times n$ .

**2. Explicit Calculation:** Let's look at the equation for just *one* element of the output, say  $y_i$  (the  $i$ -th row of  $\mathbf{y}$ ).

$$y_i = (\text{Row } i \text{ of } \mathbf{W}) \cdot \mathbf{x} + b_i$$

Written as a sum:

$$y_i = \sum_{k=1}^n W_{ik}x_k + b_i$$

Now, calculate the partial derivative of  $y_i$  with respect to a specific input  $x_j$ :

$$\frac{\partial y_i}{\partial x_j} = \frac{\partial}{\partial x_j} (W_{i1}x_1 + \cdots + W_{ij}x_j + \cdots + W_{in}x_n + b_i)$$

\*Logic Check:\*

- $b_i$  is constant w.r.t  $x_j$ . Derivative is 0.
- For any  $k \neq j$ ,  $W_{ik}x_k$  is constant w.r.t  $x_j$ . Derivative is 0.
- The only term that survives is  $W_{ij}x_j$ .

$$\frac{\partial y_i}{\partial x_j} = W_{ij}$$

\*Final Assembly:\* The entry at row  $i$ , column  $j$  of the Jacobian corresponds to  $W_{ij}$ . Therefore, the Jacobian matrix is exactly the weight matrix.

$$\mathbf{J} = \mathbf{W}$$

### Problem 3: The Element-wise Activation

Let  $\mathbf{h} \in \mathbb{R}^k$ . Let  $\mathbf{z} = \sigma(\mathbf{h})$ , where  $\sigma$  is the sigmoid function applied **element-wise** (i.e.,  $z_i = \sigma(h_i)$ ).

Compute the Jacobian matrix  $\frac{\partial \mathbf{z}}{\partial \mathbf{h}}$ . Explain why this matrix is diagonal.

#### Detailed Solution:

**1. Dimensions:** Input size  $k$ , Output size  $k$ . Jacobian is  $k \times k$ .

**2. The "Cross-Talk" Check:** We need to calculate  $\frac{\partial z_i}{\partial h_j}$ . Ask yourself: "Does changing input  $h_j$  affect output  $z_i$ ?"

- **Case A (Off-Diagonal,  $i \neq j$ ):** Since the function is element-wise,  $z_1$  depends ONLY on  $h_1$ .  $z_1$  does NOT depend on  $h_2$ . Therefore,  $\frac{\partial z_i}{\partial h_j} = 0$  for all  $i \neq j$ .
- **Case B (Diagonal,  $i = j$ ):** Here,  $z_i = \sigma(h_i)$ . This is just a standard scalar derivative.  $\frac{\partial z_i}{\partial h_i} = \sigma'(h_i)$ .

**3. Constructing the Matrix:**

$$\mathbf{J} = \begin{bmatrix} \sigma'(h_1) & 0 & \dots \\ 0 & \sigma'(h_2) & \dots \\ \vdots & \vdots & \ddots \end{bmatrix}$$

This is a diagonal matrix. In vector notation:

$$\frac{\partial \mathbf{z}}{\partial \mathbf{h}} = \text{diag}(\sigma'(\mathbf{h}))$$

### 3 Part 3: Matrix Calculus using the Trace Trick

**Time Allocation: 45 Minutes**

**The Trace Identification Theorem:** If you can manipulate the differential of a scalar  $L$  into the form:

$$dL = \text{tr}(\mathbf{G}^T d\mathbf{X})$$

Then the gradient is:

$$\nabla_{\mathbf{X}} L = \mathbf{G}$$

#### Problem 4: Trace of a Linear Product

Let  $L = \text{tr}(\mathbf{A}\mathbf{X})$ , where  $\mathbf{A}$  and  $\mathbf{X}$  are square matrices. Find  $\nabla_{\mathbf{X}} L$ .

**Detailed Solution:**

**Step 1: Take the Differential** Apply the operator  $d$  to the equation. The trace is a linear operator, so  $d$  moves inside.

$$dL = d(\text{tr}(\mathbf{A}\mathbf{X})) = \text{tr}(d(\mathbf{A}\mathbf{X}))$$

**Step 2: Apply Matrix Rules**  $\mathbf{A}$  is a constant matrix, so it does not change ( $d\mathbf{A} = 0$ ).  $\mathbf{X}$  is the variable.

$$d(\mathbf{A}\mathbf{X}) = \mathbf{A}(d\mathbf{X})$$

Substitute this back:

$$dL = \text{tr}(\mathbf{A}d\mathbf{X})$$

**Step 3: Match the Identification Form** We need the form  $\text{tr}(\mathbf{G}^T d\mathbf{X})$ . Currently we have  $\text{tr}(\mathbf{A}d\mathbf{X})$ . Set them equal to find  $\mathbf{G}$ :

$$\mathbf{G}^T = \mathbf{A}$$

Take the transpose of both sides:

$$\mathbf{G} = \mathbf{A}^T$$

**Answer:**  $\nabla_{\mathbf{X}} L = \mathbf{A}^T$ .

#### Problem 5: Trace of a Quadratic Product

Let  $L = \text{tr}(\mathbf{X}^T \mathbf{A} \mathbf{X})$ , where  $\mathbf{A}$  is a constant square matrix. Find  $\nabla_{\mathbf{X}} L$ .

**Detailed Solution:**

**Step 1: Product Rule for Differentials** Treat  $\mathbf{X}^T$ ,  $\mathbf{A}$ , and  $\mathbf{X}$  as three separate terms being multiplied. Rule:  $d(UVW) = (dU)VW + U(dV)W + UV(dW)$ . Since  $\mathbf{A}$  is constant ( $d\mathbf{A} = 0$ ), the middle term vanishes.

$$dL = \text{tr} \left( \underbrace{(d\mathbf{X}^T)}_{\text{Diff first term}} \mathbf{A} \mathbf{X} + \mathbf{X}^T \mathbf{A} \underbrace{(d\mathbf{X})}_{\text{Diff last term}} \right)$$

Note that  $d(\mathbf{X}^T) = (d\mathbf{X})^T$ .

$$dL = \text{tr}((d\mathbf{X})^T \mathbf{A} \mathbf{X} + \mathbf{X}^T \mathbf{A} d\mathbf{X})$$

**Step 2: Linearity of Trace** Split the trace of a sum into a sum of traces:

$$dL = \underbrace{\text{tr}((d\mathbf{X})^T \mathbf{A} \mathbf{X})}_{\text{Term 1}} + \underbrace{\text{tr}(\mathbf{X}^T \mathbf{A} d\mathbf{X})}_{\text{Term 2}}$$

**Step 3: The Transpose Trick (Crucial Step)** We want both terms to have  $d\mathbf{X}$  on the right side. Term 2 is already good. Term 1 has  $(d\mathbf{X})^T$ . \*Identity:\*  $\text{tr}(\mathbf{M}) = \text{tr}(\mathbf{M}^T)$ . Apply this to Term 1. Let  $\mathbf{M} = (d\mathbf{X})^T \mathbf{A} \mathbf{X}$ .

$$\mathbf{M}^T = (\mathbf{A} \mathbf{X})^T ((d\mathbf{X})^T)^T = \mathbf{X}^T \mathbf{A}^T d\mathbf{X}$$

So, Term 1 becomes:  $\text{tr}(\mathbf{X}^T \mathbf{A}^T d\mathbf{X})$ .

**Step 4: Combine Terms** Now substitute the transformed Term 1 back into the equation:

$$dL = \text{tr}(\mathbf{X}^T \mathbf{A}^T d\mathbf{X}) + \text{tr}(\mathbf{X}^T \mathbf{A} d\mathbf{X})$$

Factor out the common parts ( $\mathbf{X}^T$  at start,  $d\mathbf{X}$  at end):

$$dL = \text{tr}(\mathbf{X}^T (\mathbf{A}^T + \mathbf{A}) d\mathbf{X})$$

**Step 5: Identify the Gradient** Compare with  $dL = \text{tr}(\mathbf{G}^T d\mathbf{X})$ .

$$\mathbf{G}^T = \mathbf{X}^T (\mathbf{A}^T + \mathbf{A})$$

Take transpose of both sides (remember  $(XY)^T = Y^T X^T$ ):

$$\mathbf{G} = (\mathbf{A}^T + \mathbf{A})^T (\mathbf{X}^T)^T$$

$$\mathbf{G} = (\mathbf{A} + \mathbf{A}^T) \mathbf{X}$$

## Problem 6: Linear Regression (Normal Equation)

Let  $L = \|\mathbf{A}\mathbf{x} - \mathbf{b}\|_2^2$ . Derive  $\nabla_{\mathbf{x}} L$  and set to 0.

**Detailed Solution:**

**Step 1: Convert Norm to Trace** The squared Euclidean norm  $\|\mathbf{v}\|^2$  is equivalent to dot product  $\mathbf{v}^T \mathbf{v}$ , which is equivalent to  $\text{tr}(\mathbf{v}^T \mathbf{v})$ . Let  $\mathbf{r} = \mathbf{A}\mathbf{x} - \mathbf{b}$  (the residual vector).

$$L = \text{tr}(\mathbf{r}^T \mathbf{r})$$

**Step 2: Differentiate w.r.t the Residual  $\mathbf{r}$**  From Problem 5 (with  $\mathbf{A} = \mathbf{I}$ ), we know  $d(\text{tr}(\mathbf{r}^T \mathbf{r})) = \text{tr}(2\mathbf{r}^T d\mathbf{r})$ .

$$dL = \text{tr}(2\mathbf{r}^T d\mathbf{r})$$

**Step 3: Find  $d\mathbf{r}$**  We need to relate changes in  $\mathbf{r}$  to changes in  $\mathbf{x}$ .

$$\mathbf{r} = \mathbf{A}\mathbf{x} - \mathbf{b}$$

Apply differential:

$$d\mathbf{r} = d(\mathbf{A}\mathbf{x}) - d(\mathbf{b})$$

Since  $\mathbf{b}$  is constant,  $d\mathbf{b} = 0$ .

$$d\mathbf{r} = \mathbf{A} d\mathbf{x}$$

**Step 4: Substitute back into  $dL$**  Replace  $d\mathbf{r}$  in the equation from Step 2:

$$dL = \text{tr}(2\mathbf{r}^T (\mathbf{A} d\mathbf{x}))$$

**Step 5: Rotate/Associate to isolate  $d\mathbf{x}$**  Use matrix associativity. We want  $d\mathbf{x}$  isolated at the end.

$$dL = \text{tr}((2\mathbf{r}^T \mathbf{A}) d\mathbf{x})$$

**Step 6: Identify Gradient** Match with  $\text{tr}(\mathbf{G}^T d\mathbf{x})$ . Note that since  $\mathbf{x}$  is a vector,  $\mathbf{G}$  is a vector, so  $\mathbf{G}^T$  is a row vector.

$$\mathbf{G}^T = 2\mathbf{r}^T \mathbf{A}$$

Take transpose:

$$\mathbf{G} = (2\mathbf{r}^T \mathbf{A})^T = 2\mathbf{A}^T \mathbf{r}$$

**Step 7: Expand r** Substitute  $\mathbf{r} = \mathbf{Ax} - \mathbf{b}$  back in:

$$\nabla_{\mathbf{x}} L = 2\mathbf{A}^T (\mathbf{Ax} - \mathbf{b})$$